Optimizations MUL(X,1) and MUL(X,0) with proof.

datatypes.v
@@ -15,6 +15,7 @@ Definition WLen: nat := 256.
 Definition EVMWord:= word WLen.
 Definition StackLen := 1024.
 Definition WZero: EVMWord  := natToWord WLen 0.
+Definition WOne : EVMWord  := natToWord WLen 1.
 Definition WTrue: EVMWord  := natToWord WLen 1.
 End EVM_Def.
 Import EVM_Def.
